looking good

SystemF/lean/extrinsic/FreeTheorems.lean
@@ -7,15 +7,15 @@ def idR {A : Ty} (V : Term) : Rel A A :=
 
 theorem free_theorem_id :
   ∀ {A : Ty} (M V : Term),
-    HasType 0 [] M (.all (.fn (.var 0) (.var 0))) →
-    HasType 0 [] V A →
+    0 ⊢ [] ⊢ M ⦂ (∀ₜ (#0 ⇒ #0)) →
+    0 ⊢ [] ⊢ V ⦂ A →
     Value V →
-    Nonempty ((.app (.tapp M) V) —↠ V)
+    Nonempty (((M ∙[]) ∙ V) —↠ V)
   | A, M, V, hM, _, vV => by
-      have hRel : LogicalRel [] (.all (.fn (.var 0) (.var 0))) M M :=
+      have hRel : LogicalRel [] (∀ₜ (#0 ⇒ #0)) M M :=
         fundamental M hM
       have hEval :
-          ERel (.all (.fn (.var 0) (.var 0))) emptyRelSub
+          ERel (∀ₜ (#0 ⇒ #0)) emptyRelSub
             (subst emptyRelEnv.gamma1 M) (subst emptyRelEnv.gamma2 M) :=
         hRel emptyRelSub emptyRelEnv GRel_empty
       rcases hEval with ⟨_, _, vM, wM, mSteps, _, hAll⟩
@@ -28,7 +28,7 @@ theorem free_theorem_id :
         cases vf <;> cases wf <;> try (cases (by simpa [VRel] using hFun : False))
         case vLam.vLam =>
           have hArgRel :
-              VRel (.var 0) (extendRelSub emptyRelSub A A (idR V)) V V vV vV := by
+              VRel (#0) (extendRelSub emptyRelSub A A (idR V)) V V vV vV := by
             simp [VRel, extendRelSub, idR]
           rcases hFun vV vV hArgRel with ⟨R1, appSteps1, R2, _, _, _, hRes⟩
           rcases appSteps1 with ⟨appSteps1⟩
@@ -36,7 +36,7 @@ theorem free_theorem_id :
             multi_trans (tapp_multi mSteps) (multi_trans (beta_tlam_multi (N := _)) fSteps1)
           have hSub : subst emptyRelEnv.gamma1 M = M := by
             simpa [emptyRelEnv, id] using sub_id M
-          have hApp : (.app (.tapp M) V) —↠ R1 :=
+          have hApp : (((M ∙[]) ∙ V)) —↠ R1 :=
             multi_trans
               (app_multi (by simpa [hSub] using hTappSub) .vLam (.refl V))
               (multi_trans (beta_lam_multi vV) appSteps1)
@@ -45,70 +45,70 @@ theorem free_theorem_id :
           exact ⟨by simpa [hId.1.symm] using hApp⟩
 
 def neg : Term :=
-  .lam (.ite (.var 0) .tfalse .ttrue)
+  ƛ (ˋif ˋ0 then ˋfalse else ˋtrue)
 
 def flip : Term :=
-  .lam (.natCase (.var 0) (.suc .zero) .zero)
+  ƛ (caseₜ ˋ0 [zero⇒ (ˋsuc ˋzero) |suc⇒ ˋzero])
 
-def R : Rel .bool .nat :=
+def R : Rel 𝔹 ℕ :=
   fun V W _ _ =>
-    (V = .ttrue ∧ W = .suc .zero) ∨
-    (V = .tfalse ∧ W = .zero)
+    (V = ˋtrue ∧ W = ˋsuc ˋzero) ∨
+    (V = ˋfalse ∧ W = ˋzero)
 
 theorem neg_flip_related :
-  VRel (.fn (.var 0) (.var 0)) (extendRelSub emptyRelSub .bool .nat R) neg flip Value.vLam Value.vLam := by
+  VRel (#0 ⇒ #0) (extendRelSub emptyRelSub 𝔹 ℕ R) neg flip Value.vLam Value.vLam := by
   intro V W vV wW hVW
   have hVW' : R V W vV wW := by
     simpa [VRel, extendRelSub] using hVW
   rcases hVW' with hTrueOne | hFalseZero
   case inl =>
     rcases hTrueOne with ⟨hV, hW⟩
-    have hNeg : Nonempty (singleSubst (.ite (.var 0) .tfalse .ttrue) V —↠ .tfalse) := by
+    have hNeg : Nonempty (singleSubst (ˋif ˋ0 then ˋfalse else ˋtrue) V —↠ ˋfalse) := by
       refine ⟨?_⟩
       cases hV
       simpa [singleSubst, singleEnv, subst] using
-        (show (.ite .ttrue .tfalse .ttrue) —↠ .tfalse from
+        (show (ˋif ˋtrue then ˋfalse else ˋtrue) —↠ ˋfalse from
           .step _ .beta_true (.refl _))
-    have hFlip : Nonempty (singleSubst (.natCase (.var 0) (.suc .zero) .zero) W —↠ .zero) := by
+    have hFlip : Nonempty (singleSubst (caseₜ ˋ0 [zero⇒ (ˋsuc ˋzero) |suc⇒ ˋzero]) W —↠ ˋzero) := by
       refine ⟨?_⟩
       cases hW
       simpa [singleSubst, singleEnv, subst] using
-        (show (.natCase (.suc .zero) (.suc .zero) .zero) —↠ .zero from
+        (show (caseₜ (ˋsuc ˋzero) [zero⇒ (ˋsuc ˋzero) |suc⇒ ˋzero]) —↠ ˋzero from
           .step _ (.beta_suc .vZero) (.refl _))
-    have hR : VRel (.var 0) (extendRelSub emptyRelSub .bool .nat R) .tfalse .zero .vFalse .vZero := by
+    have hR : VRel (#0) (extendRelSub emptyRelSub 𝔹 ℕ R) ˋfalse ˋzero .vFalse .vZero := by
       simpa [VRel, extendRelSub, R]
-    exact ⟨Term.tfalse, Term.zero, Value.vFalse, Value.vZero, hNeg, hFlip, hR⟩
+    exact ⟨ˋfalse, ˋzero, Value.vFalse, Value.vZero, hNeg, hFlip, hR⟩
   case inr =>
     rcases hFalseZero with ⟨hV, hW⟩
-    have hNeg : Nonempty (singleSubst (.ite (.var 0) .tfalse .ttrue) V —↠ .ttrue) := by
+    have hNeg : Nonempty (singleSubst (ˋif ˋ0 then ˋfalse else ˋtrue) V —↠ ˋtrue) := by
       refine ⟨?_⟩
       cases hV
       simpa [singleSubst, singleEnv, subst] using
-        (show (.ite .tfalse .tfalse .ttrue) —↠ .ttrue from
+        (show (ˋif ˋfalse then ˋfalse else ˋtrue) —↠ ˋtrue from
           .step _ .beta_false (.refl _))
-    have hFlip : Nonempty (singleSubst (.natCase (.var 0) (.suc .zero) .zero) W —↠ (.suc .zero)) := by
+    have hFlip : Nonempty (singleSubst (caseₜ ˋ0 [zero⇒ (ˋsuc ˋzero) |suc⇒ ˋzero]) W —↠ (ˋsuc ˋzero)) := by
       refine ⟨?_⟩
       cases hW
       simpa [singleSubst, singleEnv, subst] using
-        (show (.natCase .zero (.suc .zero) .zero) —↠ (.suc .zero) from
+        (show (caseₜ ˋzero [zero⇒ (ˋsuc ˋzero) |suc⇒ ˋzero]) —↠ (ˋsuc ˋzero) from
           .step _ .beta_zero (.refl _))
-    have hR : VRel (.var 0) (extendRelSub emptyRelSub .bool .nat R) .ttrue (.suc .zero) .vTrue (.vSuc .vZero) := by
+    have hR : VRel (#0) (extendRelSub emptyRelSub 𝔹 ℕ R) ˋtrue (ˋsuc ˋzero) .vTrue (.vSuc .vZero) := by
       simpa [VRel, extendRelSub, R]
-    exact ⟨Term.ttrue, (Term.suc Term.zero), Value.vTrue, (Value.vSuc Value.vZero), hNeg, hFlip, hR⟩
+    exact ⟨ˋtrue, ˋsuc ˋzero, Value.vTrue, (Value.vSuc Value.vZero), hNeg, hFlip, hR⟩
 
 theorem free_theorem_rep :
   ∀ (M : Term),
-    HasType 0 [] M (.all (.fn (.var 0) (.fn (.fn (.var 0) (.var 0)) (.var 0)))) →
+    0 ⊢ [] ⊢ M ⦂ (∀ₜ (#0 ⇒ ((#0 ⇒ #0) ⇒ #0)) ) →
     ∃ V, ∃ W, ∃ (v : Value V), ∃ (w : Value W),
-      Nonempty ((.app (.app (.tapp M) .ttrue) neg) —↠ V) ∧
-      Nonempty ((.app (.app (.tapp M) (.suc .zero)) flip) —↠ W) ∧
+      Nonempty ((((M ∙[]) ∙ ˋtrue) ∙ neg) —↠ V) ∧
+      Nonempty ((((M ∙[]) ∙ (ˋsuc ˋzero)) ∙ flip) —↠ W) ∧
       R V W v w
   | M, hM => by
       have hRel :
-          LogicalRel [] (.all (.fn (.var 0) (.fn (.fn (.var 0) (.var 0)) (.var 0)))) M M :=
+          LogicalRel [] (∀ₜ (#0 ⇒ ((#0 ⇒ #0) ⇒ #0)) ) M M :=
         fundamental M hM
       have hEval :
-          ERel (.all (.fn (.var 0) (.fn (.fn (.var 0) (.var 0)) (.var 0)))) emptyRelSub
+          ERel (∀ₜ (#0 ⇒ ((#0 ⇒ #0) ⇒ #0)) ) emptyRelSub
             (subst emptyRelEnv.gamma1 M) (subst emptyRelEnv.gamma2 M) :=
         hRel emptyRelSub emptyRelEnv GRel_empty
       rcases hEval with ⟨_, _, vM, wM, mSteps, nSteps, hAll⟩
@@ -117,14 +117,14 @@ theorem free_theorem_rep :
       cases vM <;> cases wM <;> simp [VRel] at hAll
       case vTlam.vTlam =>
         rename_i N1 N2
-        rcases hAll .bool .nat R with ⟨F1, fSteps1, F2, fSteps2, vf, wf, hFun⟩
+        rcases hAll 𝔹 ℕ R with ⟨F1, fSteps1, F2, fSteps2, vf, wf, hFun⟩
         rcases fSteps1 with ⟨fSteps1⟩
         rcases fSteps2 with ⟨fSteps2⟩
         cases vf <;> cases wf <;> try (cases (by simpa [VRel] using hFun : False))
         case vLam.vLam =>
           have hArgRel :
-              VRel (.var 0) (extendRelSub emptyRelSub .bool .nat R)
-                .ttrue (.suc .zero) .vTrue (.vSuc .vZero) := by
+              VRel (#0) (extendRelSub emptyRelSub 𝔹 ℕ R)
+                ˋtrue (ˋsuc ˋzero) .vTrue (.vSuc .vZero) := by
             simpa [VRel, extendRelSub, R]
           rcases hFun .vTrue (.vSuc .vZero) hArgRel with
             ⟨G1, gSteps1, G2, gSteps2, vg, wg, hFun2⟩
@@ -134,14 +134,14 @@ theorem free_theorem_rep :
           case vLam.vLam =>
             have hNegFlipArg :
                 ∀ {V' W' : Term} (v' : Value V') (w' : Value W'),
-                  (extendRelSub emptyRelSub .bool .nat R).rhoR 0 V' W' v' w' →
+                  (extendRelSub emptyRelSub 𝔹 ℕ R).rhoR 0 V' W' v' w' →
                     ∃ VB,
-                      Nonempty (singleSubst (.ite (.var 0) .tfalse .ttrue) V' —↠ VB) ∧
+                      Nonempty (singleSubst (ˋif ˋ0 then ˋfalse else ˋtrue) V' —↠ VB) ∧
                         ∃ x,
-                          Nonempty (singleSubst (.natCase (.var 0) (.suc .zero) .zero) W' —↠ x) ∧
-                            ∃ x_1 x_2, (extendRelSub emptyRelSub .bool .nat R).rhoR 0 VB x x_1 x_2 := by
+                          Nonempty (singleSubst (caseₜ ˋ0 [zero⇒ (ˋsuc ˋzero) |suc⇒ ˋzero]) W' —↠ x) ∧
+                            ∃ x_1 x_2, (extendRelSub emptyRelSub 𝔹 ℕ R).rhoR 0 VB x x_1 x_2 := by
               intro V' W' v' w' hR0
-              have hRelV : VRel (.var 0) (extendRelSub emptyRelSub .bool .nat R) V' W' v' w' := by
+              have hRelV : VRel (#0) (extendRelSub emptyRelSub 𝔹 ℕ R) V' W' v' w' := by
                 simpa [VRel, extendRelSub] using hR0
               rcases neg_flip_related v' w' hRelV with
                 ⟨VB, WB, vb, wb, hL, hR, hVW⟩
@@ -158,9 +158,9 @@ theorem free_theorem_rep :
               have hTapp :=
                 multi_trans (tapp_multi mSteps) (multi_trans (beta_tlam_multi (N := _)) fSteps1)
               exact multi_trans
-                (app_multi hTapp .vLam (.refl .ttrue))
+                (app_multi hTapp .vLam (.refl ˋtrue))
                 (multi_trans (beta_lam_multi .vTrue) gSteps1)
-            have hAppL2Sub : (.app (.app (.tapp (subst emptyRelEnv.gamma1 M)) .ttrue) neg) —↠ Vres := by
+            have hAppL2Sub : ((((subst emptyRelEnv.gamma1 M) ∙[]) ∙ ˋtrue) ∙ neg) —↠ Vres := by
               exact multi_trans
                 (app_multi hAppL1Sub .vLam (.refl neg))
                 (multi_trans (beta_lam_multi .vLam) resSteps1)
@@ -168,15 +168,15 @@ theorem free_theorem_rep :
               have hTapp :=
                 multi_trans (tapp_multi nSteps) (multi_trans (beta_tlam_multi (N := _)) fSteps2)
               exact multi_trans
-                (app_multi hTapp .vLam (.refl (.suc .zero)))
+                (app_multi hTapp .vLam (.refl (ˋsuc ˋzero)))
                 (multi_trans (beta_lam_multi (.vSuc .vZero)) gSteps2)
-            have hAppR2Sub : (.app (.app (.tapp (subst emptyRelEnv.gamma2 M)) (.suc .zero)) flip) —↠ Wres := by
+            have hAppR2Sub : ((((subst emptyRelEnv.gamma2 M) ∙[]) ∙ (ˋsuc ˋzero)) ∙ flip) —↠ Wres := by
               exact multi_trans
                 (app_multi hAppR1Sub .vLam (.refl flip))
                 (multi_trans (beta_lam_multi .vLam) resSteps2)
-            have hAppL2 : (.app (.app (.tapp M) .ttrue) neg) —↠ Vres := by
+            have hAppL2 : ((((M ∙[]) ∙ ˋtrue) ∙ neg) —↠ Vres) := by
               simpa [hSub1] using hAppL2Sub
-            have hAppR2 : (.app (.app (.tapp M) (.suc .zero)) flip) —↠ Wres := by
+            have hAppR2 : ((((M ∙[]) ∙ (ˋsuc ˋzero)) ∙ flip) —↠ Wres) := by
               simpa [hSub2] using hAppR2Sub
             have hR : R Vres Wres vRes wRes := by
               simpa [VRel, extendRelSub] using hRes
