SystemF/lean/extrinsic/Reduction.lean
@@ -3,47 +3,47 @@ import extrinsic.Terms
 namespace Extrinsic
 
 inductive Value : Term → Type where
-  | vLam {N} : Value (.lam N)
-  | vTrue : Value .ttrue
-  | vFalse : Value .tfalse
-  | vZero : Value .zero
-  | vSuc {V} : Value V → Value (.suc V)
-  | vTlam {N} : Value (.tlam N)
+  | vLam {N} : Value (ƛ N)
+  | vTrue : Value ˋtrue
+  | vFalse : Value ˋfalse
+  | vZero : Value ˋzero
+  | vSuc {V} : Value V → Value (ˋsuc V)
+  | vTlam {N} : Value (Λ N)
 
 inductive Step : Term → Term → Type where
   | xi_app₁ {L L' M} :
       Step L L' →
-      Step (.app L M) (.app L' M)
+      Step (L ∙ M) (L' ∙ M)
   | xi_app₂ {V M M'} :
       Value V →
       Step M M' →
-      Step (.app V M) (.app V M')
+      Step (V ∙ M) (V ∙ M')
   | beta_lam {N W} :
       Value W →
-      Step (.app (.lam N) W) (singleSubst N W)
+      Step ((ƛ N) ∙ W) (singleSubst N W)
   | xi_suc {M M'} :
       Step M M' →
-      Step (.suc M) (.suc M')
+      Step (ˋsuc M) (ˋsuc M')
   | xi_if {L L' M N} :
       Step L L' →
-      Step (.ite L M N) (.ite L' M N)
+      Step (ˋif L then M else N) (ˋif L' then M else N)
   | xi_case {L L' M N} :
       Step L L' →
-      Step (.natCase L M N) (.natCase L' M N)
+      Step (caseₜ L [zero⇒ M |suc⇒ N]) (caseₜ L' [zero⇒ M |suc⇒ N])
   | beta_true {M N} :
-      Step (.ite .ttrue M N) M
+      Step (ˋif ˋtrue then M else N) M
   | beta_false {M N} :
-      Step (.ite .tfalse M N) N
+      Step (ˋif ˋfalse then M else N) N
   | beta_zero {M N} :
-      Step (.natCase .zero M N) M
+      Step (caseₜ ˋzero [zero⇒ M |suc⇒ N]) M
   | beta_suc {V M N} :
       Value V →
-      Step (.natCase (.suc V) M N) (singleSubst N V)
+      Step (caseₜ (ˋsuc V) [zero⇒ M |suc⇒ N]) (singleSubst N V)
   | xi_tapp {M M'} :
       Step M M' →
-      Step (.tapp M) (.tapp M')
+      Step (M ∙[]) (M' ∙[])
   | beta_tlam {N} :
-      Step (.tapp (.tlam N)) N
+      Step ((Λ N) ∙[]) N
 
 inductive MultiStep : Term → Term → Type where
   | refl (M) : MultiStep M M
@@ -62,14 +62,14 @@ def multi_trans {M N L : Term} :
   | step K hK hKN ih => exact .step K hK (ih h₂)
 
 def app_right_multi {V M M' : Term} :
-    Value V → M —↠ M' → (.app V M) —↠ (.app V M') := by
+    Value V → M —↠ M' → (V ∙ M) —↠ (V ∙ M') := by
   intro vV h
   induction h with
   | refl => exact .refl _
   | step K hK hKN ih => exact .step _ (.xi_app₂ vV hK) ih
 
 def app_multi {L L' M M' : Term} :
-    L —↠ L' → Value L' → M —↠ M' → (.app L M) —↠ (.app L' M') := by
+    L —↠ L' → Value L' → M —↠ M' → (L ∙ M) —↠ (L' ∙ M') := by
   intro hL vL hM
   induction hL generalizing M M' with
   | refl =>
@@ -78,61 +78,61 @@ def app_multi {L L' M M' : Term} :
       exact .step _ (.xi_app₁ hK) (ih (M := M) (M' := M') vL hM)
 
 def suc_multi {M N : Term} :
-    M —↠ N → (.suc M) —↠ (.suc N) := by
+    M —↠ N → (ˋsuc M) —↠ (ˋsuc N) := by
   intro h
   induction h with
   | refl => exact .refl _
   | step K hK hKN ih => exact .step _ (.xi_suc hK) ih
 
 def case_multi {L L' M N : Term} :
-    L —↠ L' → (.natCase L M N) —↠ (.natCase L' M N) := by
+    L —↠ L' → (caseₜ L [zero⇒ M |suc⇒ N]) —↠ (caseₜ L' [zero⇒ M |suc⇒ N]) := by
   intro h
   induction h with
   | refl => exact .refl _
   | step K hK hKN ih => exact .step _ (.xi_case hK) ih
 
 def if_true_multi_aux {L T M N : Term} :
-    L —↠ T → T = .ttrue → (.ite L M N) —↠ M
+    L —↠ T → T = ˋtrue → (ˋif L then M else N) —↠ M
   | .refl _, hT => by
       cases hT
       exact .step _ .beta_true (.refl _)
   | .step K hK hKT, hT =>
       .step _ (.xi_if hK) (if_true_multi_aux hKT hT)
 
-def if_true_multi {L M N : Term} : L —↠ .ttrue → (.ite L M N) —↠ M := by
+def if_true_multi {L M N : Term} : L —↠ ˋtrue → (ˋif L then M else N) —↠ M := by
   intro h
   exact if_true_multi_aux h rfl
 
 def if_false_multi_aux {L T M N : Term} :
-    L —↠ T → T = .tfalse → (.ite L M N) —↠ N
+    L —↠ T → T = ˋfalse → (ˋif L then M else N) —↠ N
   | .refl _, hT => by
       cases hT
       exact .step _ .beta_false (.refl _)
   | .step K hK hKF, hT =>
       .step _ (.xi_if hK) (if_false_multi_aux hKF hT)
 
-def if_false_multi {L M N : Term} : L —↠ .tfalse → (.ite L M N) —↠ N := by
+def if_false_multi {L M N : Term} : L —↠ ˋfalse → (ˋif L then M else N) —↠ N := by
   intro h
   exact if_false_multi_aux h rfl
 
 def tapp_multi {M M' : Term} :
-    M —↠ M' → (.tapp M) —↠ (.tapp M') := by
+    M —↠ M' → (M ∙[]) —↠ (M' ∙[]) := by
   intro h
   induction h with
   | refl => exact .refl _
   | step K hK hKN ih => exact .step _ (.xi_tapp hK) ih
 
 def beta_lam_multi {N W : Term} :
-    Value W → (.app (.lam N) W) —↠ singleSubst N W := by
+    Value W → ((ƛ N) ∙ W) —↠ singleSubst N W := by
   intro vW
   exact .step _ (.beta_lam vW) (.refl _)
 
 def case_zero_multi {M N : Term} :
-    (.natCase .zero M N) —↠ M := by
+    (caseₜ ˋzero [zero⇒ M |suc⇒ N]) —↠ M := by
   exact .step _ .beta_zero (.refl _)
 
 def beta_tlam_multi {N : Term} :
-    (.tapp (.tlam N)) —↠ N := by
+    ((Λ N) ∙[]) —↠ N := by
   exact .step _ .beta_tlam (.refl _)
 
 end
