SystemF/lean/extrinsic/Types.lean
@@ -11,49 +11,74 @@ inductive Ty where
   | all  : Ty → Ty
   deriving DecidableEq, Repr
 
+syntax "#" num : term
+syntax "#" ident : term
+syntax "#(" term ")" : term
+macro_rules
+  | `(#$n:num) => `(Ty.var $n)
+  | `(#$x:ident) => `(Ty.var $x)
+  | `(#($t:term)) => `(Ty.var $t)
+
+@[match_pattern] abbrev ℕ : Ty := Ty.nat
+@[match_pattern] abbrev 𝔹 : Ty := Ty.bool
 infixr:60 " ⇒ " => Ty.fn
+prefix:80 "∀ₜ " => Ty.all
 
 abbrev Ctx : Type := List Ty
 
 abbrev RenameT : Type := Var → Var
 abbrev SubstT : Type := Var → Ty
+abbrev Renameₜ : Type := RenameT
+abbrev Substₜ : Type := SubstT
 
 def extT (ρ : RenameT) : RenameT
   | 0 => 0
   | i + 1 => (ρ i) + 1
 
+abbrev extₜ := extT
+
 def renameT (ρ : RenameT) : Ty → Ty
-  | .var i => .var (ρ i)
-  | .nat => .nat
-  | .bool => .bool
-  | .fn A B => .fn (renameT ρ A) (renameT ρ B)
-  | .all A => .all (renameT (extT ρ) A)
+  | #i => #(ρ i)
+  | ℕ => ℕ
+  | 𝔹 => 𝔹
+  | A ⇒ B => (renameT ρ A) ⇒ (renameT ρ B)
+  | ∀ₜ A => ∀ₜ (renameT (extT ρ) A)
+
+abbrev renameₜ := renameT
 
 def extsT (σ : SubstT) : SubstT
-  | 0 => .var 0
+  | 0 => #0
   | i + 1 => renameT Nat.succ (σ i)
 
+abbrev extsₜ := extsT
+
 def substT (σ : SubstT) : Ty → Ty
-  | .var i => σ i
-  | .nat => .nat
-  | .bool => .bool
-  | .fn A B => .fn (substT σ A) (substT σ B)
-  | .all A => .all (substT (extsT σ) A)
+  | #i => σ i
+  | ℕ => ℕ
+  | 𝔹 => 𝔹
+  | A ⇒ B => (substT σ A) ⇒ (substT σ B)
+  | ∀ₜ A => ∀ₜ (substT (extsT σ) A)
+
+abbrev substₜ := substT
 
 def singleTyEnv (B : Ty) : SubstT
   | 0 => B
-  | i + 1 => .var i
+  | i + 1 => #i
 
 def substOneT (A B : Ty) : Ty :=
   substT (singleTyEnv B) A
 
-def idT : SubstT := Ty.var
+notation:67 A " [ " B " ]ₜ" => substOneT A B
+
+def idT : SubstT := fun i => #i
+abbrev idₜ : Substₜ := idT
 
 def consSubT (A : Ty) (σ : SubstT) : SubstT
   | 0 => A
   | i + 1 => σ i
 
 infixr:61 " •ᵗ " => consSubT
+infixr:61 " •ₜ " => consSubT
 
 def substCtx (σ : SubstT) : Ctx → Ctx
   | [] => []
@@ -62,12 +87,14 @@ def substCtx (σ : SubstT) : Ctx → Ctx
 def liftCtx (Γ : Ctx) : Ctx :=
   Γ.map (renameT Nat.succ)
 
+prefix:100 "⤊" => liftCtx
+
 inductive WfTy : TyCtx → Ty → Type where
-  | var  {Δ X} : X < Δ → WfTy Δ (.var X)
-  | nat  {Δ}   : WfTy Δ .nat
-  | bool {Δ}   : WfTy Δ .bool
+  | var  {Δ X} : X < Δ → WfTy Δ (#X)
+  | nat  {Δ}   : WfTy Δ ℕ
+  | bool {Δ}   : WfTy Δ 𝔹
   | fn   {Δ A B} : WfTy Δ A → WfTy Δ B → WfTy Δ (.fn A B)
-  | all  {Δ A} : WfTy (Δ + 1) A → WfTy Δ (.all A)
+  | all  {Δ A} : WfTy (Δ + 1) A → WfTy Δ (∀ₜ A)
 
 inductive HasTypeVar : Ctx → Var → Ty → Type where
   | Z {Γ A} : HasTypeVar (A :: Γ) 0 A
