SystemF/lean/SystemF.lean
@@ -6,12 +6,10 @@ import extrinsic.Progress
 import extrinsic.Preservation
 import extrinsic.TypeSafety
 import extrinsic.Eval
-import extrinsic.ProductOmega
 import extrinsic.LogicalRelation
 import extrinsic.Parametricity
 import extrinsic.FreeTheorems
 import extrinsic.Examples
-import extrinsic.SystemF
 
 namespace SystemF
 
